\documentclass[11pt,letterpaper]{article}
\usepackage[english]{babel}
\usepackage[utf8]{inputenc}
\usepackage{fancyhdr}
\usepackage[margin=1in]{geometry}
\usepackage{enumitem}
\usepackage{amsmath}
\usepackage{graphicx}
\usepackage{setspace} 
\onehalfspacing
 
\pagestyle{fancy}
\fancyhf{}
\lhead{STAT 435 HW 1}
\rhead{Nan Tang (1662478)}
\rfoot{Page \thepage}
 

\title{STAT 435 Homework 1}
\author{Nan Tang 1662478}
\date{\today}

\begin{document}
\section*{part2 - a}

\begin{align*}
D &= E(\frac{1}{n} \| f - \hat{f} \|^2 ) \\
&= E(\frac{1}{n} \| f - E(\hat{f}) - \hat{f} + E(\hat{f})\|^2 ) \\
&= E(\frac{1}{n} \| f - E(\hat{f}) - \hat{f} + E(\hat{f})\|^2 ) \\
&= \frac{1}{n} [E(\| f - E(\hat{f}) \|^2) + E(\| \hat{f} - E(\hat{f}) \|^2)  + 2E(E(\| f - E(\hat{f}) \|) E(\| \hat{f} - E(\hat{f} ) \|)]
\end{align*}

\noindent Note that $E(E(\|\hat{f} - E(\hat{f}) \|)) = 0$, two terms are independent to each other, therefore the cross term $2E(E(\| f - E(\hat{f}) \|) E(\| \hat{f} - E(\hat{f} ) \|) = 0$.
\begin{align*}
D &= \frac{1}{n} [E(\| f - E(\hat{f}) \|^2) + E(\| \hat{f} - E(\hat{f}) \|^2) ]
\end{align*}

\noindent Separately write two terms. \\

\noindent Since $\hat{f} = W y$ and $y = f + \epsilon$, where $y, f, \epsilon$ are vectors, $E(\hat{f}) = E(W y) = W E(f + \epsilon ) = W f$ 

\begin{align*}
E(\| f - E(\hat{f}) \|^2) &= E(\| f - Wf \|^2) \\
&= E(\| (W-I) f \|^2)
\end{align*}
\noindent Since $W$ depends only on bandwidth, and $f$ is parameter, this term can be written as $\| (W-I) f \|^2$\\


\noindent $E(\| \hat{f} - E(\hat{f}) \|^2)$ is the variance of $\| \hat{f} \|$, where $\hat{f} = W y$. 
\begin{align*}
E(\| \hat{f} - E(\hat{f}) \|^2) &= Var(\| W \| y ) \\
&= \| W^2 \| Var(y) \\
&= trace(W^T W) \sigma^2
\end{align*}

\noindent Combine these two term, we proved:
\begin{align*}
D &= \frac{1}{n} (\| (W-I) f \|^2 + trace(W^T W) \sigma^2 )
\end{align*}

\end{document}